verify/Skelet34.v
@@ -1,0 +1,108 @@
+(** * Skelet #34 *)
+
+(** Following https://www.sligocki.com/2023/02/02/skelet-34.html *)
+
+Set Warnings "-notation-overriden,-parsing,-deprecated-hint-without-locality".
+From Coq Require Import List. Import ListNotations.
+From Coq Require Import PArith.BinPos.
+From Coq Require Import NArith.BinNat.
+From BusyCoq Require Import Extraction. Import ETranslatedCyclers.
+Set Default Goal Selector "!".
+
+Notation "0" := S0.
+Notation "1" := S1.
+Notation side := (Stream sym).
+
+Definition tm : TM := fun '(q, s) =>
+  match q, s with
+  | A, 0 => Some (1, R, B)  | A, 1 => Some (1, L, C)
+  | B, 0 => Some (0, R, C)  | B, 1 => Some (0, R, B)
+  | C, 0 => Some (1, L, D)  | C, 1 => Some (0, L, A)
+  | D, 0 => Some (1, L, E)  | D, 1 => None
+  | E, 0 => Some (1, L, A)  | E, 1 => Some (1, R, A)
+  end.
+
+(** Trivial lemmas, but [simpl] in these situations leaves a mess. *)
+Lemma move_left_const : forall s0 s r,
+  move_left (const s0 {{s}} r) = const s0 {{s0}} s >> r.
+Proof. reflexivity. Qed.
+
+Lemma move_right_const : forall l s s0,
+  move_right (l {{s}} const s0) = l << s {{s0}} const s0.
+Proof. reflexivity. Qed.
+
+(** [assumption] and [eassumption] both refuse to instantiate [forall]s. *)
+
+Ltac apply_assumption :=
+  match goal with
+  | H: _ |- _ => apply H
+  end.
+
+Ltac prove_step_left := apply step_left; reflexivity.
+Ltac prove_step_right := apply step_right; reflexivity.
+Ltac prove_step := prove_step_left || prove_step_right.
+Ltac simpl_tape :=
+  try rewrite move_left_const;
+  try rewrite move_right_const;
+  simpl.
+Ltac step := eapply evstep_step; [prove_step | simpl_tape].
+Ltac execute := repeat step; try apply evstep_refl.
+Ltac follow_assm := eapply evstep_trans; [apply_assumption; assumption |].
+Ltac follow_hyp H := eapply evstep_trans; [apply H; assumption |].
+
+Tactic Notation "follow" := follow_assm.
+Tactic Notation "follow" constr(H) := follow_hyp H.
+
+Ltac triv := introv; repeat (step || follow); try apply evstep_refl.
+
+Notation "c --> c'" := (c -[ tm ]-> c')   (at level 40).
+Notation "c -->* c'" := (c -[ tm ]->* c') (at level 40).
+Notation "l <{{ q }} r" := (q; tl l {{hd l}} r)  (at level 30, q at next level).
+Notation "l {{ q }}> r" := (q; l {{hd r}} tl r)  (at level 30, q at next level).
+
+Fixpoint L (n : positive) : side :=
+  match n with
+  | xH => const 0 << 1 << 0 << 0 << 0
+  | xO n => L n << 0 << 0 << 0 << 0
+  | xI n => L n << 1 << 0 << 0 << 0
+  end.
+
+Fixpoint R (n : positive) : side :=
+  match n with
+  | xH => 1 >> 1 >> const 0
+  | xO n => 1 >> 0 >> R n
+  | xI n => 1 >> 1 >> R n
+  end.
+
+Definition counter (n m : positive) : Q * tape :=
+  L n <{{C}} 1 >> 0 >> 1 >> 0 >> R m.
+
+Lemma left_inc : forall n r,
+  L n <{{C}} r -->* L (Pos.succ n) {{B}}> r.
+Proof.
+  induction n; triv.
+Qed.
+
+Inductive has0 : positive -> Prop :=
+  | has0_0 n: has0 (n~0)
+  | has0_1 n: has0 n -> has0 (n~1).
+
+Inductive all1 : positive -> Prop :=
+  | all1_H:   all1 1
+  | all1_1 n: all1 n -> all1 (n~1).
+
+Lemma right_inc_has0 : forall n l,
+  has0 n ->
+  l << 0 {{C}}> R n -->* l <{{A}} 0 >> R (Pos.succ n).
+Proof.
+  introv H. generalize dependent l. induction H; triv.
+Qed.
+
+Corollary counter_inc : forall n m,
+  has0 m ->
+  counter n m -->* counter (Pos.succ n) (Pos.succ m).
+Proof.
+  introv H. unfold counter.
+  follow left_inc. execute.
+  follow right_inc_has0. execute.
+Qed.
